variable renaming
To be consistent with the paper, I renamed variables as follows:

- stack variables: s
- state variables: q
- code continuation variables c, sc/fc (for two continuations approach)

ExceptionsTwoCont.v
@@ -38,12 +38,12 @@ Inductive Code : Set :=
 | POP : Code -> Code
 | HALT : Code.
 
-Fixpoint comp' (e : Expr) (s : Code) (f : Code) : Code :=
+Fixpoint comp' (e : Expr) (sc : Code) (fc : Code) : Code :=
   match e with
-    | Val n =>  PUSH n s
-    | Add x y => comp' x (comp' y (ADD s) (POP f)) f 
-    | Throw => f
-    | Catch x h => comp' x s (comp' h s f)
+    | Val n =>  PUSH n sc
+    | Add x y => comp' x (comp' y (ADD sc) (POP fc)) fc 
+    | Throw => fc
+    | Catch x h => comp' x sc (comp' h sc fc)
   end.
 
 Definition comp (e : Expr) : Code := comp' e HALT HALT.
@@ -62,9 +62,9 @@ Notation "⟨ x , y ⟩" := (conf x y).
 
 Reserved Notation "x ==> y" (at level 80, no associativity).
 Inductive VM : Conf -> Conf -> Prop :=
-| vm_push n c k : ⟨PUSH n c, k⟩ ==> ⟨ c , VAL n :: k ⟩
-| vm_add c k m n : ⟨ADD c, VAL m :: VAL n :: k⟩ ==> ⟨c, VAL (n + m) :: k⟩
-| vm_pop c n k : ⟨POP c, VAL n :: k⟩ ==> ⟨c, k⟩
+| vm_push n c s : ⟨PUSH n c, s⟩ ==> ⟨ c , VAL n :: s ⟩
+| vm_add c s m n : ⟨ADD c, VAL m :: VAL n :: s⟩ ==> ⟨c, VAL (n + m) :: s⟩
+| vm_pop c n s : ⟨POP c, VAL n :: s⟩ ==> ⟨c, s⟩
 where "x ==> y" := (VM x y).
 
 Hint Constructors VM.
@@ -82,19 +82,19 @@ Import VMCalc.
 
 (** Specification of the compiler *)
 
-Theorem spec e s f k : ⟨comp' e s f, k⟩
+Theorem spec e sc fc s : ⟨comp' e sc fc, s⟩
                        =>> match eval e with
-                            | Some n => ⟨s , VAL n :: k⟩
-                            | None => ⟨f , k⟩
+                            | Some n => ⟨sc , VAL n :: s⟩
+                            | None => ⟨fc , s⟩
                            end.
 
 (** Setup the induction proof *)
 
 Proof.
   intros.
+  generalize dependent sc.
+  generalize dependent fc.
   generalize dependent s.
-  generalize dependent f.
-  generalize dependent k.
   induction e;intros.
 
 (** Calculation of the compiler *)
@@ -102,9 +102,9 @@ Proof.
 (** - [e = Val n]: *)
 
   begin
-  ⟨s, VAL n :: k⟩.
+  ⟨sc, VAL n :: s⟩.
   <== { apply vm_push }
-  ⟨PUSH n s, k⟩.
+  ⟨PUSH n sc, s⟩.
   [].
 
 (** - [e = Add e1 e2]: *)
@@ -112,59 +112,59 @@ Proof.
   begin
    (match eval e1 with
      | Some m => match eval e2 with
-                  | Some n => ⟨ s, VAL (m + n) :: k ⟩
-                  | None => ⟨ f, k ⟩
+                  | Some n => ⟨ sc, VAL (m + n) :: s ⟩
+                  | None => ⟨ fc, s ⟩
                   end
-     | None => ⟨ f, k ⟩
+     | None => ⟨ fc, s ⟩
      end).
   <<= { apply vm_add }
    (match eval e1 with
      | Some m => match eval e2 with
-                  | Some n => ⟨ ADD s, VAL n :: VAL m :: k ⟩
-                  | None => ⟨ f, k ⟩
+                  | Some n => ⟨ ADD sc, VAL n :: VAL m :: s ⟩
+                  | None => ⟨ fc, s ⟩
                   end
-     | None => ⟨ f, k ⟩
+     | None => ⟨ fc, s ⟩
      end).
   <<= { apply vm_pop }
    (match eval e1 with
      | Some m => match eval e2 with
-                  | Some n => ⟨ ADD s, VAL n :: VAL m :: k ⟩
-                  | None => ⟨ POP f, VAL m :: k ⟩
+                  | Some n => ⟨ ADD sc, VAL n :: VAL m :: s ⟩
+                  | None => ⟨ POP fc, VAL m :: s ⟩
                   end
-     | None => ⟨ f, k ⟩
+     | None => ⟨ fc, s ⟩
      end).
   <<= { apply IHe2 }
    (match eval e1 with
-     | Some m =>  ⟨ (comp' e2 (ADD s) (POP f)), VAL m :: k⟩
-     | None => ⟨ f, k ⟩
+     | Some m =>  ⟨ (comp' e2 (ADD sc) (POP fc)), VAL m :: s⟩
+     | None => ⟨ fc, s ⟩
      end).
   <<= { apply IHe1 }
-      ⟨ comp' e1 (comp' e2 (ADD s) (POP f)) f, k ⟩.
+      ⟨ comp' e1 (comp' e2 (ADD sc) (POP fc)) fc, s ⟩.
   [].
 
 (** - [e = Throw]: *)
 
   begin
-    ⟨ f, k⟩.
+    ⟨ fc, s⟩.
   [].
 
 (** - [e = Catch e1 e2]: *)
 
   begin
     (match eval e1 with
-         | Some m => ⟨ s, VAL m :: k⟩
+         | Some m => ⟨ sc, VAL m :: s⟩
          | None => match eval e2 with
-                     | Some n => ⟨s, VAL n :: k⟩
-                     | None => ⟨f, k⟩
+                     | Some n => ⟨sc, VAL n :: s⟩
+                     | None => ⟨fc, s⟩
                    end
     end).
    <<= { apply IHe2 }
     (match eval e1 with
-         | Some m => ⟨ s, VAL m :: k⟩
-         | None => ⟨comp' e2 s f, k⟩
+         | Some m => ⟨ sc, VAL m :: s⟩
+         | None => ⟨comp' e2 sc fc, s⟩
     end).
    <<= { apply IHe1 }
-       ⟨ comp' e1 s (comp' e2 s f) , k⟩.
+       ⟨ comp' e1 sc (comp' e2 sc fc) , s⟩.
    [].
 Qed.
 
